@prefix wfprov: <http://purl.org/wf4ever/wfprov#> .
@prefix xsd: <http://www.w3.org/2001/XMLSchema#> .
@prefix owl: <http://www.w3.org/2002/07/owl#> .
@prefix rdfg: <http://www.w3.org/2004/03/trix/rdfg-1/> .
@prefix ore: <http://www.openarchives.org/ore/terms/> .
@prefix : <http://www.semanticweb.org/owl/owlapi/turtle#> .
@prefix xml: <http://www.w3.org/XML/1998/namespace> .
@prefix rdf: <http://www.w3.org/1999/02/22-rdf-syntax-ns#> .
@prefix rdfs: <http://www.w3.org/2000/01/rdf-schema#> .
@prefix dct: <http://purl.org/dc/terms/> .
@prefix ro: <http://purl.org/wf4ever/ro#> .
@prefix ao: <http://purl.org/ao/> .
@base <http://purl.org/wf4ever/ro> .

<http://purl.org/wf4ever/ro> rdf:type owl:Ontology ;
                             
                             rdfs:comment "This ontology shows how AO and ORE ontologies can be used together to define a ResearchObject. This ontology is further customized by the wf4ever ontology."@en ;
                             
                             owl:imports <http://purl.org/dc/terms/> ,
                                         <http://purl.org/ao/core/> ,
                                         <http://purl.org/wf4ever/ore-owl> ;
                             
                             rdfs:seeAlso <http://www.wf4ever-project.org/wiki/display/docs/Research+Object+Vocabulary+Specification> ;
                             
                             owl:imports <http://xmlns.com/foaf/0.1/> ;
                             
                             owl:versionIRI <https://raw.github.com/wf4ever/ro/master/ro.owl> .


#################################################################
#
#    Annotation properties
#
#################################################################




#################################################################
#
#    Datatypes
#
#################################################################




#################################################################
#
#    Object Properties
#
#################################################################

# Copied from http://bloody-byte.net/rdf/dc_owl2dl/dcterms_od.ttl


dcterms:created a owl:DatatypeProperty ;
	rdfs:label "Date Created"@en-us ;
	skos:definition "Date of creation of the resource."@en-us ;
	rdfs:subPropertyOf dcterms:date ;
	rdfs:range rdfs:Literal .

dcterms:creator a owl:ObjectProperty ;
	rdfs:label "Creator"@en-us ;
	skos:definition "An entity primarily responsible for making the resource."@en-us ;
	rdfs:comment "Examples of a Creator include a person, an organization, or a service. Typically, the name of a Creator should be used to indicate the entity."@en-us ;
	rdfs:subPropertyOf dcterms:contributor ;
	rdfs:range dcterms:Agent .

dcterms:date a owl:DatatypeProperty ;
	rdfs:label "Date"@en-us ;
	skos:definition "A point or period of time associated with an event in the lifecycle of the resource."@en-us ;
	rdfs:comment "Date may be used to express temporal information at any level of granularity. Recommended best practice is to use an encoding scheme, such as the W3CDTF profile of ISO 8601 [W3CDTF]."@en-us ;
	dcterms:bibliographicCitation "[W3CDTF] http://www.w3.org/TR/NOTE-datetime" ;
	rdfs:seeAlso <http://www.w3.org/TR/NOTE-datetime> ;
	rdfs:range rdfs:Literal .


dcterms:contributor a owl:ObjectProperty ;
	rdfs:label "Contributor"@en-us ;
	skos:definition "An entity responsible for making contributions to the resource."@en-us ;
	rdfs:comment "Examples of a Contributor include a person, an organization, or a service. Typically, the name of a Contributor should be used to indicate the entity."@en-us ;
	rdfs:range dcterms:Agent .

dcterms:Agent a owl:Class , dcterms:AgentClass ;
	rdfs:label "Agent"@en-us ;
	skos:definition "A resource that acts or has the power to act."@en-us ;
	rdfs:comment "Examples of Agent include person, organization, and software agent."@en-us .

dcterms:AgentClass a owl:Class ;
	rdfs:label "Agent Class"@en-us ;
	skos:definition "A group of agents."@en-us ;
	rdfs:comment "Examples of Agent Class include groups seen as classes, such as students, women, charities, lecturers."@en-us .
#	rdfs:subClassOf rdfs:Class . # Not allowed in OWL 2 DL, neither rdfs:Class nor owl:Class.    


#################################################################
#
#    Data properties
#
#################################################################


###  http://purl.org/wf4ever/ro#entryName

ro:entryName rdf:type owl:DatatypeProperty ,
                      owl:FunctionalProperty ;
             
             rdfs:comment """This functional property specifies the name of a ro:FolderEntry within an ro:Folder. 

This name must be case-sensitively unique within the ro:Folder, similar to a filename in a directory.

TODO: Need a functional property to specify the top level folder structure of an {{ro:ResearchObject}}?
"""@en ;
             
             rdfs:domain ro:FolderEntry ;
             
             rdfs:range xsd:string .





#################################################################
#
#    Classes
#
#################################################################


###  http://purl.org/wf4ever/ro#Annotation

ro:Annotation rdf:type owl:Class ;
                        
                        rdfs:subClassOf ao:GraphAnnotation ,
                                        ore:AggregatedResource ,
                                        [ rdf:type owl:Restriction ;
                                          owl:onProperty ore:isAggregatedBy ;
                                          owl:someValuesFrom ro:ResearchObject
                                        ] ,
                                        [ rdf:type owl:Restriction ;
                                          owl:onProperty <http://purl.org/ao/annotatesResource> ;
                                          owl:someValuesFrom [ rdf:type owl:Class ;
                                                               owl:unionOf ( ro:ResearchObject
                                                                             ore:AggregatedResource
                                                                             ore:Proxy
                                                                           )
                                                             ]
                                        ] ,
                                        [ rdf:type owl:Restriction ;
                                          owl:onProperty dct:created ;
                                          owl:someValuesFrom xsd:dateTime
                                        ] ,
                                        [ rdf:type owl:Restriction ;
                                          owl:onProperty dct:creator ;
                                          owl:someValuesFrom <http://xmlns.com/foaf/0.1/Agent>
                                        ] ;
                        
                        rdfs:comment """An annotation aggregated within an ro:ResearchObject.  

Instances of this class are used to annotated resources aggregated within the aggregating research object, proxies of these resources, or the research object itself. In other words, if :ro is the ro:ResearchObject this annotation has been ore:isAggregatedBy, then the annotation should have at least one ao:annotatesResource which is an ore:AggregatedResource which is ore:isAggregatedBy :ro, or the annotated resource is an ore:Proxy which ore:proxyIn :ro, or the annotated resource is :ro.

It is possible for the annotation to also annotate non-aggregated resources, but as above, at least one of them needs to be part of the RO or the RO itself.

As a subclass of ao:GraphAnnotation the ao:body must point to an rdfg:Graph which contains the actual annotation. """@en .



###  http://purl.org/wf4ever/ro#Folder

ro:Folder rdf:type owl:Class ;
          
          rdfs:subClassOf ro:Resource ,
                          ore:Aggregation ;
          
          rdfs:comment """An ro:Folder is a special kind of ore:Aggregation where every ro:AggregatedResource must have a ro:FolderEntry proxy with a unique ro:entryName within that folder.

Note that all resources which are aggregated within an (potentially nested) ro:Folder SHOULD also be aggregated by the same ro:ResearchObject this ro:Folder is aggregated within.

Such folders can be nested and (optionally) used to organize the resources of the research object into a file-like structure. All such resources should also be aggregated by the ro:ResearchObject
          """@en .



###  http://purl.org/wf4ever/ro#FolderEntry

ro:FolderEntry rdf:type owl:Class ;
               
               owl:equivalentClass [ rdf:type owl:Restriction ;
                                     owl:onProperty ro:entryName ;
                                     owl:someValuesFrom xsd:string
                                   ] ,
                                   [ rdf:type owl:Restriction ;
                                     owl:onProperty ore:proxyIn ;
                                     owl:someValuesFrom ro:Folder
                                   ] ;
               
               rdfs:subClassOf ore:Proxy ;
               
               rdfs:comment "An ro:FolderEntry is any ore:Proxy instance that associates a resources aggregated within an ro:Folder with a ro:entryName. This name is (case-sensitive) unique within a given folder."@en ;
               
               owl:hasKey ( ore:proxyIn
                            ro:entryName
                          ) .



###  http://purl.org/wf4ever/ro#Manifest

ro:Manifest rdf:type owl:Class ;
            
            owl:equivalentClass [ rdf:type owl:Restriction ;
                                  owl:onProperty ore:describes ;
                                  owl:someValuesFrom ro:ResearchObject
                                ] ;
            
            rdfs:subClassOf ore:ResourceMap ;
            
            rdfs:comment "The ro:Manifest is used to describe an ro:ResearchObject. This identifies the resource for the manifest which lists all the aggregations of the research object, typically called \".ro/manifest.rdf\" relative to the research object this manifest ore:describes."@en .



###  http://purl.org/wf4ever/ro#ResearchObject

ro:ResearchObject rdf:type owl:Class ;
                  
                  owl:equivalentClass [ rdf:type owl:Restriction ;
                                        owl:onProperty ore:isDescribedBy ;
                                        owl:someValuesFrom ro:Manifest
                                      ] ;
                  
                  rdfs:subClassOf ore:Aggregation ,
                                  [ rdf:type owl:Restriction ;
                                    owl:onProperty dct:created ;
                                    owl:someValuesFrom xsd:dateTime
                                  ] ,
                                  [ rdf:type owl:Restriction ;
                                    owl:onProperty dct:creator ;
                                    owl:someValuesFrom <http://xmlns.com/foaf/0.1/Agent>
                                  ] ;
                  
                  rdfs:comment "A research object aggregates a number of resources. A resource can be a workflow, web service, document, data item, data set, workflow run, software or a research object."@en .



###  http://purl.org/wf4ever/ro#Resource

ro:Resource rdf:type owl:Class ;
            
            rdfs:subClassOf ore:AggregatedResource ,
                            [ rdf:type owl:Restriction ;
                              owl:onProperty ore:isAggregatedBy ;
                              owl:someValuesFrom ro:ResearchObject
                            ] ,
                            [ rdf:type owl:Restriction ;
                              owl:onProperty [ owl:inverseOf ore:proxyFor
                                             ] ;
                              owl:someValuesFrom [ rdf:type owl:Restriction ;
                                                   owl:onProperty ore:proxyIn ;
                                                   owl:someValuesFrom ro:ResearchObject
                                                 ]
                            ] ;
            
            rdfs:comment """An ro:Resource is an ore:AggregatedResource which ore:isAggregatedBy an ro:ResearchObject. 

This specialisation requires that there exists an ore:Proxy which is ore:proxyFor this resource, and which is ore:proxyIn the same ro:ResearchObject the resource ore:isAggregatedBy. Any annotations on such a proxy will descrive the ro:Resource within that particular ro:ResearchObject, in particular dct:creator and dct:created on the proxy will specify who added the resource to the aggregation at what time.

Note that annotations (ro:Annotation) can be added to both the ro:Resource and the ore:Proxy - depending on if the annotation is seen to be globally true (such as the provenance of how the resource was created) or locally true within the Research Object (such as the the resource playing the role of a wf4ever:Dataset).

Not all resources aggregated by an ro:ResearchObject are ro:Resource instances, in particular ro:Annotations will also be aggregated, but are not required to also be ro:Resources (needing their own ore:Proxy).  

Aggregated resources MAY also be organised in (potentially nested) ro:Folders to reflect a file-system like structure. Note that any such resources SHOULD also be aggregated in the \"mother\" ro:ResearchObject.
"""@en .




###  Generated by the OWL API (version 3.2.3.1824) http://owlapi.sourceforge.net

