
<!-- Processed by Id: cwm.py,v 1.197 2007/12/13 15:38:39 syosi Exp -->
<!--     using base file:///home/stain/stuff/src/wf4ever/ro/wf4ever.owl-->


<rdf:RDF xmlns="http://www.w3.org/2002/07/owl#"
    xmlns:owl="http://www.w3.org/2002/07/owl#"
    xmlns:rdf="http://www.w3.org/1999/02/22-rdf-syntax-ns#"
    xmlns:rdfs="http://www.w3.org/2000/01/rdf-schema#">

    <Ontology rdf:about="http://purl.org/wf4ever/wf4ever">
        <rdfs:comment xml:lang="en">The wf4ever ontology. This is based on the wf4ever ontologies ro, wf and wfprov - but adds custom classes like wf4ever:Image and wf4ever:WebServiceProcess</rdfs:comment>
        <imports rdf:resource="http://purl.org/wf4ever/ro"/>
        <imports rdf:resource="http://purl.org/wf4ever/wfdesc"/>
        <imports rdf:resource="http://purl.org/wf4ever/wfprov"/>
        <versionIRI rdf:resource="https://raw.github.com/wf4ever/ro/master/wf4ever.owl"/>
    </Ontology>

    <Class rdf:about="http://purl.org/wf4ever/wf4ever#Dataset">
        <rdfs:subClassOf rdf:resource="http://purl.org/wf4ever/wfdesc#Artifact"/>
    </Class>

    <Class rdf:about="http://purl.org/wf4ever/wf4ever#Document">
        <rdfs:subClassOf rdf:resource="http://purl.org/wf4ever/wfdesc#Artifact"/>
    </Class>

    <Class rdf:about="http://purl.org/wf4ever/wf4ever#File">
        <rdfs:subClassOf rdf:resource="http://purl.org/wf4ever/wfdesc#Artifact"/>
    </Class>

    <Class rdf:about="http://purl.org/wf4ever/wf4ever#Image">
        <rdfs:subClassOf rdf:resource="http://purl.org/wf4ever/wfdesc#Artifact"/>
    </Class>

    <Class rdf:about="http://purl.org/wf4ever/wf4ever#WebServiceProcess">
        <rdfs:comment>WebServiceProcess is a wfdesc:Process description, the enactment of which gives rise to a web service call.</rdfs:comment>
        <rdfs:subClassOf rdf:resource="http://purl.org/wf4ever/wfdesc#Process"/>
    </Class>

    <Class rdf:about="http://purl.org/wf4ever/wf4ever#WorkflowResearchObject">
        <rdfs:comment>A workflow research object is a research object that contains at least one workflow description.</rdfs:comment>
        <equivalentClass rdf:parseType="Resource">
            <rdf:type rdf:resource="http://www.w3.org/2002/07/owl#Class"/>
            <intersectionOf rdf:parseType="Resource">
                <rdf:first rdf:resource="http://purl.org/wf4ever/ro#ResearchObject"/>
                <rdf:rest rdf:parseType="Resource">
                    <rdf:first rdf:parseType="Resource">
                        <rdf:type rdf:resource="http://www.w3.org/2002/07/owl#Restriction"/>
                        <onProperty rdf:resource="http://www.openarchives.org/ore/terms/aggregates"/>
                        <someValuesFrom rdf:resource="http://purl.org/wf4ever/wfdesc#Workflow"/>
                    </rdf:first>
                    <rdf:rest rdf:resource="http://www.w3.org/1999/02/22-rdf-syntax-ns#nil"/>
                </rdf:rest>
            </intersectionOf>
        </equivalentClass>
    </Class>
</rdf:RDF>
