@prefix xsd: <http://www.w3.org/2001/XMLSchema#> .
@prefix owl: <http://www.w3.org/2002/07/owl#> .
@prefix opm: <http://purl.org/net/opmv/ns#> .
@prefix wf: <http://www.wf4ever-project.org/vocab/wf#> .
@prefix : <http://www.wf4ever-project.org/vocab/wfprov#> .
@prefix xml: <http://www.w3.org/XML/1998/namespace> .
@prefix rdf: <http://www.w3.org/1999/02/22-rdf-syntax-ns#> .
@prefix rdfs: <http://www.w3.org/2000/01/rdf-schema#> .
@base <http://www.wf4ever-project.org/vocab/wfprov> .

<http://www.wf4ever-project.org/vocab/wfprov> rdf:type owl:Ontology ;
                                            
                                            owl:imports <http://purl.org/net/opmv/ns> ,
                                                        <http://www.wf4ever-project.org/vocab/wf> .


#################################################################
#
#    Annotation properties
#
#################################################################




#################################################################
#
#    Datatypes
#
#################################################################




#################################################################
#
#    Object Properties
#
#################################################################


:instanceOfArtifactTemplate rdf:type owl:ObjectProperty ;
                     
                     rdfs:comment "This object property is used to associate an artifact to its correponding template."@en ;
                     
                     rdfs:domain opm:Artifact ;
                     
                     rdfs:range wf:ArtifactTemplate .



:instanceOfProcessTemplate rdf:type owl:ObjectProperty ;
                    
                    rdfs:comment "This object property associate a process to its template."@en ;
                    
                    rdfs:domain opm:Process ;
                    
                    rdfs:range wf:ProcessTemplate .



:instanceOfWorkflowTemplate rdf:type owl:ObjectProperty ;
                     
                     rdfs:comment "This property associates a workflow run to its corresponding workflow template."@en ;
                     
                     rdfs:domain :WorkflowRun ;
                     
                     rdfs:subPropertyOf :instanceOfProcessTemplate;
                     
                     rdfs:range wf:WorkflowTemplate .



###  http://www.wf4ever-project.org/vocab/wfprov#wasEnactedBy

:wasEnactedBy rdf:type owl:ObjectProperty ;
              
              rdfs:comment "wasEnactedBy associates a process with a workflow engine, specifying that the execution of the former was enacted by the latter."@en ;
              
              rdfs:subPropertyOf opm:wasControlledBy ;
              
              rdfs:range :WorkflowEngine .



###  http://www.wf4ever-project.org/vocab/wfprov#wasPartOfWorkflowRun

:wasPartOfWorkflowRun rdf:type owl:ObjectProperty ;
                      
                      rdfs:comment "This property associates a workflow run with a process to specify that the latter is a constituent of the former."@en ;
                      rdfs:domain opm:Process ; 
                      rdfs:range :WorkflowRun .



###  http://www.wf4ever-project.org/vocab/wfprov#wasSpecifiedUsing

:wasSpecifiedUsing rdf:type owl:ObjectProperty ;
                   
                   rdfs:comment "This object property is used to specify the workflow workbench using which a given workflow template was specified."@en ;
                   
                   rdfs:subPropertyOf owl:topObjectProperty ;
                   
                   rdfs:range :WorkflowEditor ;
                   
                   rdfs:domain wf:WorkflowTemplate .





#################################################################
#
#    Classes
#
#################################################################


###  http://www.wf4ever-project.org/vocab/wfprov#Tool

:Tool rdf:type owl:Class ;
      
      rdfs:subClassOf opm:Agent ;
      
      rdfs:comment "A software program (which can act as an opm:Agent/foaf:Agent)"@en .



###  http://www.wf4ever-project.org/vocab/wfprov#WorkflowEditor

:WorkflowEditor rdf:type owl:Class ;
                
                rdfs:subClassOf :Tool ;
                
                rdfs:comment "A workflow editor is a software program that provides designers with a a means to write Workflow Templates."@en ;
                
                rdfs:seeAlso wf:WorkflowTemplate .



###  http://www.wf4ever-project.org/vocab/wfprov#WorkflowEngine

:WorkflowEngine rdf:type owl:Class ;
                
                rdfs:subClassOf :Tool ;
                
                rdfs:comment "A workflow engine is an egent that is responsible for enacting a given workflow template. The result of workflow enactment gives rise to a workflow run."@en ;
                
                rdfs:seeAlso :WorkflowRun .



###  http://www.wf4ever-project.org/vocab/wfprov#WorkflowRun

:WorkflowRun rdf:type owl:Class ;
             
             rdfs:subClassOf opm:Process ;
             
             rdfs:comment "A workflow run is a Process which have been enacted by a Workflow Engine, according to the execution definition from a Workflow Template. Such a process typically contains several subprocesses corresponding to Process Definitions"@en ;
             
             rdfs:seeAlso :WorkflowEngine ,
                          wf:ProcessTemplate ,
                          wf:WorkflowTemplate .




###  Generated by the OWL API (version 3.2.3.1824) http://owlapi.sourceforge.net

