<?xml version="1.0"?>


<!DOCTYPE rdf:RDF [
    <!ENTITY ao "http://purl.org/ao/" >
    <!ENTITY foaf "http://xmlns.com/foaf/0.1/" >
    <!ENTITY ns "http://purl.org/net/opmv/ns#" >
    <!ENTITY owl "http://www.w3.org/2002/07/owl#" >
    <!ENTITY xsd "http://www.w3.org/2001/XMLSchema#" >
    <!ENTITY rdfs "http://www.w3.org/2000/01/rdf-schema#" >
    <!ENTITY terms "http://www.openarchives.org/ore/terms/" >
    <!ENTITY ro "http://www.wf4ever-project.org/vocab/ro#" >
    <!ENTITY rdf "http://www.w3.org/1999/02/22-rdf-syntax-ns#" >
    <!ENTITY dcmi-terms "http://dublincore.org/documents/dcmi-terms/" >
]>


<rdf:RDF xmlns="http://www.wf4ever-project.org/vocab/ro#"
     xml:base="http://www.wf4ever-project.org/vocab/ro"
     xmlns:dcmi-terms="http://dublincore.org/documents/dcmi-terms/"
     xmlns:rdfs="http://www.w3.org/2000/01/rdf-schema#"
     xmlns:ro="http://www.wf4ever-project.org/vocab/ro#"
     xmlns:ns="http://purl.org/net/opmv/ns#"
     xmlns:foaf="http://xmlns.com/foaf/0.1/"
     xmlns:ao="http://purl.org/ao/"
     xmlns:terms="http://www.openarchives.org/ore/terms/"
     xmlns:owl="http://www.w3.org/2002/07/owl#"
     xmlns:xsd="http://www.w3.org/2001/XMLSchema#"
     xmlns:rdf="http://www.w3.org/1999/02/22-rdf-syntax-ns#">
    <owl:Ontology rdf:about="http://www.wf4ever-project.org/vocab/ro">
        <owl:imports rdf:resource="http://purl.org/ao/"/>
        <owl:imports rdf:resource="http://www.openarchives.org/ore/terms/"/>
    </owl:Ontology>
    


    <!-- 
    ///////////////////////////////////////////////////////////////////////////////////////
    //
    // Annotation properties
    //
    ///////////////////////////////////////////////////////////////////////////////////////
     -->

    <owl:AnnotationProperty rdf:about="&rdfs;seeAlso"/>
    <owl:AnnotationProperty rdf:about="&rdfs;label"/>
    <owl:AnnotationProperty rdf:about="&rdfs;comment"/>
    <owl:AnnotationProperty rdf:about="&dcmi-terms;creator"/>
    


    <!-- 
    ///////////////////////////////////////////////////////////////////////////////////////
    //
    // Datatypes
    //
    ///////////////////////////////////////////////////////////////////////////////////////
     -->

    


    <!-- http://www.w3.org/1999/02/22-rdf-syntax-ns#PlainLiteral -->

    <rdfs:Datatype rdf:about="&rdf;PlainLiteral"/>
    


    <!-- 
    ///////////////////////////////////////////////////////////////////////////////////////
    //
    // Object Properties
    //
    ///////////////////////////////////////////////////////////////////////////////////////
     -->

    


    <!-- http://purl.org/ao/annotatesResource -->

    <owl:ObjectProperty rdf:about="&ao;annotatesResource"/>
    


    <!-- http://purl.org/ao/body -->

    <owl:ObjectProperty rdf:about="&ao;body"/>
    


    <!-- http://purl.org/net/opmv/ns#used -->

    <owl:ObjectProperty rdf:about="&ns;used">
        <rdfs:comment>used associates an artifact with a process, specifying that the former was consumed by the latter.</rdfs:comment>
        <rdfs:range rdf:resource="&ns;Artifact"/>
        <rdfs:domain rdf:resource="&ns;Process"/>
        <rdfs:subPropertyOf rdf:resource="&owl;topObjectProperty"/>
    </owl:ObjectProperty>
    


    <!-- http://purl.org/net/opmv/ns#wasControlledBy -->

    <owl:ObjectProperty rdf:about="&ns;wasControlledBy">
        <rdfs:comment>wasControlledBy associates a process with an agent, specifying the process  was controlled, e.g., launched, suspended, or terminated, by the agent.</rdfs:comment>
        <rdfs:range rdf:resource="&ns;Agent"/>
        <rdfs:domain rdf:resource="&ns;Process"/>
        <rdfs:subPropertyOf rdf:resource="&owl;topObjectProperty"/>
    </owl:ObjectProperty>
    


    <!-- http://purl.org/net/opmv/ns#wasGeneratedBy -->

    <owl:ObjectProperty rdf:about="&ns;wasGeneratedBy">
        <rdfs:comment>wasGeneratedBy associates an artifact with a process, specifying that the former was produced by the latter.</rdfs:comment>
        <rdfs:domain rdf:resource="&ns;Artifact"/>
        <rdfs:range rdf:resource="&ns;Process"/>
        <rdfs:subPropertyOf rdf:resource="&owl;topObjectProperty"/>
    </owl:ObjectProperty>
    


    <!-- http://www.openarchives.org/ore/terms/aggregates -->

    <owl:ObjectProperty rdf:about="&terms;aggregates"/>
    


    <!-- http://www.w3.org/2002/07/owl#topObjectProperty -->

    <owl:ObjectProperty rdf:about="&owl;topObjectProperty"/>
    


    <!-- http://www.wf4ever-project.org/vocab/ro#contains -->

    <owl:ObjectProperty rdf:about="&ro;contains">
        <rdfs:comment>This property associates a workflow run with a process to specify that the latter is a constituent of the former.</rdfs:comment>
        <rdfs:range rdf:resource="&ns;Process"/>
        <rdfs:subPropertyOf rdf:resource="&owl;topObjectProperty"/>
        <rdfs:domain rdf:resource="&ro;WorkflowRun"/>
    </owl:ObjectProperty>
    


    <!-- http://www.wf4ever-project.org/vocab/ro#hasArtifactTemplate -->

    <owl:ObjectProperty rdf:about="&ro;hasArtifactTemplate">
        <rdfs:comment>This object property is used to associate an artifact to its correponding template.</rdfs:comment>
        <rdfs:domain rdf:resource="&ns;Artifact"/>
        <rdfs:subPropertyOf rdf:resource="&owl;topObjectProperty"/>
        <rdfs:range rdf:resource="&ro;ArtifactTemplate"/>
    </owl:ObjectProperty>
    


    <!-- http://www.wf4ever-project.org/vocab/ro#hasInput -->

    <owl:ObjectProperty rdf:about="&ro;hasInput">
        <rdfs:comment>This object property is used to specify the template of the artifacts used as input to a given process template.</rdfs:comment>
        <rdfs:range rdf:resource="&ro;ArtifactTemplate"/>
        <rdfs:domain rdf:resource="&ro;ProcessTemplate"/>
    </owl:ObjectProperty>
    


    <!-- http://www.wf4ever-project.org/vocab/ro#hasOutput -->

    <owl:ObjectProperty rdf:about="&ro;hasOutput">
        <rdfs:comment>This object property is used to specify the template of the artifacts used as output to a given process template.</rdfs:comment>
        <rdfs:range rdf:resource="&ro;ArtifactTemplate"/>
        <rdfs:domain rdf:resource="&ro;ProcessTemplate"/>
    </owl:ObjectProperty>
    


    <!-- http://www.wf4ever-project.org/vocab/ro#hasProcessTemplate -->

    <owl:ObjectProperty rdf:about="&ro;hasProcessTemplate">
        <rdfs:comment>This object property associate a process to its template.</rdfs:comment>
        <rdfs:domain rdf:resource="&ns;Process"/>
        <rdfs:subPropertyOf rdf:resource="&owl;topObjectProperty"/>
        <rdfs:range rdf:resource="&ro;ProcessTemplate"/>
    </owl:ObjectProperty>
    


    <!-- http://www.wf4ever-project.org/vocab/ro#hasWorkflowTemplate -->

    <owl:ObjectProperty rdf:about="&ro;hasWorkflowTemplate">
        <rdfs:comment>This property associates a workflow run to its corresponding workflow template.</rdfs:comment>
        <rdfs:domain rdf:resource="&ro;WorkflowRun"/>
        <rdfs:range rdf:resource="&ro;WorkflowTemplate"/>
        <rdfs:subPropertyOf rdf:resource="&ro;hasProcessTemplate"/>
    </owl:ObjectProperty>
    


    <!-- http://www.wf4ever-project.org/vocab/ro#isPartOf -->

    <owl:ObjectProperty rdf:about="&ro;isPartOf">
        <rdfs:comment rdf:datatype="&rdf;PlainLiteral">This object property is used to specify that a given process template is part of a given workflow template.</rdfs:comment>
        <rdfs:subPropertyOf rdf:resource="&owl;topObjectProperty"/>
        <rdfs:domain rdf:resource="&ro;ProcessTemplate"/>
        <rdfs:range rdf:resource="&ro;WorkflowTemplate"/>
    </owl:ObjectProperty>
    


    <!-- http://www.wf4ever-project.org/vocab/ro#isSubWorkflowOf -->

    <owl:ObjectProperty rdf:about="&ro;isSubWorkflowOf">
        <rdfs:comment>This object property is used to associate a workflow template to another workflow template, specifying that the former is a sub-workflow of the latter.</rdfs:comment>
        <rdfs:range rdf:resource="&ro;WorkflowTemplate"/>
        <rdfs:domain rdf:resource="&ro;WorkflowTemplate"/>
        <rdfs:subPropertyOf rdf:resource="&ro;isPartOf"/>
    </owl:ObjectProperty>
    


    <!-- http://www.wf4ever-project.org/vocab/ro#wasEnactedBy -->

    <owl:ObjectProperty rdf:about="&ro;wasEnactedBy">
        <rdfs:comment>wasEnactedBy associates a process with a workflow engine, specifying that the execution of the former was enacted by the latter.</rdfs:comment>
        <rdfs:subPropertyOf rdf:resource="&ns;wasControlledBy"/>
        <rdfs:range>
            <owl:Restriction>
                <owl:onProperty rdf:resource="&ro;wasEnactedBy"/>
                <owl:someValuesFrom rdf:resource="&ro;WorkflowEngine"/>
            </owl:Restriction>
        </rdfs:range>
        <rdfs:domain>
            <owl:Restriction>
                <owl:onProperty rdf:resource="&ro;wasEnactedBy"/>
                <owl:someValuesFrom rdf:resource="&ns;Process"/>
            </owl:Restriction>
        </rdfs:domain>
    </owl:ObjectProperty>
    


    <!-- http://www.wf4ever-project.org/vocab/ro#wasSpecifiedUsing -->

    <owl:ObjectProperty rdf:about="&ro;wasSpecifiedUsing">
        <rdfs:comment>This object property is used to specify the workflow workbench using which a given workflow template was specified.</rdfs:comment>
        <rdfs:subPropertyOf rdf:resource="&owl;topObjectProperty"/>
        <rdfs:domain rdf:resource="&ro;WorkflowTemplate"/>
        <rdfs:range rdf:resource="&ro;WorkflowWorkbench"/>
    </owl:ObjectProperty>
    


    <!-- 
    ///////////////////////////////////////////////////////////////////////////////////////
    //
    // Classes
    //
    ///////////////////////////////////////////////////////////////////////////////////////
     -->

    


    <!-- http://purl.org/ao/Annotation -->

    <owl:Class rdf:about="&ao;Annotation"/>
    


    <!-- http://purl.org/net/opmv/ns#Agent -->

    <owl:Class rdf:about="&ns;Agent">
        <owl:equivalentClass rdf:resource="&foaf;Agent"/>
        <rdfs:comment>An agent represents the entity that can be used to control the execution of a process, is used to specify a workflow template, or is responsible for enacting a workflow run. </rdfs:comment>
    </owl:Class>
    


    <!-- http://purl.org/net/opmv/ns#Artifact -->

    <owl:Class rdf:about="&ns;Artifact">
        <rdfs:comment>Artifact is a general concept that represents immutable piece of state, which may have a physical embodiment in a physical object, or a digital representation in a computer system. Note, however, that in the context of the Wf4ever project, the focus is on artifact that are digital representations in a computer system.</rdfs:comment>
    </owl:Class>
    


    <!-- http://purl.org/net/opmv/ns#Process -->

    <owl:Class rdf:about="&ns;Process">
        <rdfs:comment>Process refers to an action that may consume some existing arifacts, and may produce some new artifacts.</rdfs:comment>
    </owl:Class>
    


    <!-- http://www.openarchives.org/ore/terms/Aggregation -->

    <owl:Class rdf:about="&terms;Aggregation"/>
    


    <!-- http://www.openarchives.org/ore/terms/ResourceMap -->

    <owl:Class rdf:about="&terms;ResourceMap"/>
    


    <!-- http://www.w3.org/2002/07/owl#Thing -->

    <owl:Class rdf:about="&owl;Thing"/>
    


    <!-- http://www.wf4ever-project.org/vocab/ro#ArtifactTemplate -->

    <owl:Class rdf:about="&ro;ArtifactTemplate">
        <rdfs:comment>ArtifactTemplate is used to provide information about a class of artifacts. For example, it can be used to specify the datatype of a dataset or the structure of a document.</rdfs:comment>
    </owl:Class>
    


    <!-- http://www.wf4ever-project.org/vocab/ro#Dataset -->

    <owl:Class rdf:about="&ro;Dataset">
        <rdfs:subClassOf rdf:resource="&ns;Artifact"/>
    </owl:Class>
    


    <!-- http://www.wf4ever-project.org/vocab/ro#Document -->

    <owl:Class rdf:about="&ro;Document">
        <rdfs:subClassOf rdf:resource="&ns;Artifact"/>
    </owl:Class>
    


    <!-- http://www.wf4ever-project.org/vocab/ro#File -->

    <owl:Class rdf:about="&ro;File">
        <rdfs:subClassOf rdf:resource="&ns;Artifact"/>
    </owl:Class>
    


    <!-- http://www.wf4ever-project.org/vocab/ro#Image -->

    <owl:Class rdf:about="&ro;Image">
        <rdfs:subClassOf rdf:resource="&ns;Artifact"/>
    </owl:Class>
    


    <!-- http://www.wf4ever-project.org/vocab/ro#Manifest -->

    <owl:Class rdf:about="&ro;Manifest">
        <rdfs:subClassOf rdf:resource="&terms;ResourceMap"/>
        <rdfs:comment>Manifest is used to describe a research object.</rdfs:comment>
    </owl:Class>
    


    <!-- http://www.wf4ever-project.org/vocab/ro#ProcessTemplate -->

    <owl:Class rdf:about="&ro;ProcessTemplate">
        <rdfs:comment>A process template is used to describe a class of actions that when enacted give rise to processes. </rdfs:comment>
    </owl:Class>
    


    <!-- http://www.wf4ever-project.org/vocab/ro#ResearchObject -->

    <owl:Class rdf:about="&ro;ResearchObject">
        <rdfs:subClassOf rdf:resource="&terms;Aggregation"/>
        <rdfs:comment>A research object aggregates a number of resources. A resource can be a workflow, web service, document, data item, data set, workflow run, software or a research object.</rdfs:comment>
    </owl:Class>
    


    <!-- http://www.wf4ever-project.org/vocab/ro#Tool -->

    <owl:Class rdf:about="&ro;Tool">
        <rdfs:subClassOf rdf:resource="&ns;Agent"/>
        <rdfs:comment>represents a software program</rdfs:comment>
    </owl:Class>
    


    <!-- http://www.wf4ever-project.org/vocab/ro#WebServiceProcess -->

    <owl:Class rdf:about="&ro;WebServiceProcess">
        <rdfs:subClassOf rdf:resource="&ro;ProcessTemplate"/>
        <rdfs:comment>WebServiceProcess is a Process template, the enactment of which gives rise to a web service call.</rdfs:comment>
    </owl:Class>
    


    <!-- http://www.wf4ever-project.org/vocab/ro#WorkflowEngine -->

    <owl:Class rdf:about="&ro;WorkflowEngine">
        <rdfs:subClassOf rdf:resource="&ro;Tool"/>
        <rdfs:comment>A workflow engine is an egent that is responsible for enacting a given workflow template. The result of workflow enactment gives rise to a workflow run.</rdfs:comment>
    </owl:Class>
    


    <!-- http://www.wf4ever-project.org/vocab/ro#WorkflowResearchObject -->

    <owl:Class rdf:about="&ro;WorkflowResearchObject">
        <owl:equivalentClass>
            <owl:Class>
                <owl:intersectionOf rdf:parseType="Collection">
                    <rdf:Description rdf:about="&ro;ResearchObject"/>
                    <owl:Restriction>
                        <owl:onProperty rdf:resource="&terms;aggregates"/>
                        <owl:someValuesFrom rdf:resource="&ro;WorkflowTemplate"/>
                    </owl:Restriction>
                </owl:intersectionOf>
            </owl:Class>
        </owl:equivalentClass>
        <rdfs:comment>A workflow research object is a research object that contains at least one workflow template.</rdfs:comment>
    </owl:Class>
    


    <!-- http://www.wf4ever-project.org/vocab/ro#WorkflowRun -->

    <owl:Class rdf:about="&ro;WorkflowRun">
        <rdfs:subClassOf rdf:resource="&ns;Process"/>
        <rdfs:comment>A workflow run is a special kind of process that is composed of a series of actions.</rdfs:comment>
    </owl:Class>
    


    <!-- http://www.wf4ever-project.org/vocab/ro#WorkflowTemplate -->

    <owl:Class rdf:about="&ro;WorkflowTemplate">
        <rdfs:subClassOf rdf:resource="&ro;ProcessTemplate"/>
        <rdfs:comment>A workflow template is a directed graph in which the nodes are process templates and the edges represent data dependencies between the constituent process templates.</rdfs:comment>
    </owl:Class>
    


    <!-- http://www.wf4ever-project.org/vocab/ro#WorkflowWorkbench -->

    <owl:Class rdf:about="&ro;WorkflowWorkbench">
        <rdfs:subClassOf rdf:resource="&ro;Tool"/>
        <rdfs:comment>A workflow workbench is a software program that provides designers with a a means to design workflow templates.</rdfs:comment>
    </owl:Class>
    


    <!-- http://xmlns.com/foaf/0.1/Agent -->

    <owl:Class rdf:about="&foaf;Agent"/>
    


    <!-- 
    ///////////////////////////////////////////////////////////////////////////////////////
    //
    // Individuals
    //
    ///////////////////////////////////////////////////////////////////////////////////////
     -->

    


    <!-- http://www.wf4ever-project.org/vocab/ro#annotation-1 -->

    <owl:NamedIndividual rdf:about="&ro;annotation-1">
        <rdf:type rdf:resource="&ao;Annotation"/>
        <ao:body rdf:resource="&ro;annotationBody-1"/>
        <dcmi-terms:creator rdf:resource="&ro;user-18933"/>
        <ao:annotatesResource rdf:resource="&ro;workflow-run"/>
    </owl:NamedIndividual>
    


    <!-- http://www.wf4ever-project.org/vocab/ro#annotation-2 -->

    <owl:NamedIndividual rdf:about="&ro;annotation-2">
        <rdf:type rdf:resource="&ao;Annotation"/>
        <ao:body rdf:resource="&ro;annotationBody-2"/>
        <dcmi-terms:creator rdf:resource="&ro;user-18933"/>
        <ao:annotatesResource rdf:resource="&ro;workflow-run"/>
    </owl:NamedIndividual>
    


    <!-- http://www.wf4ever-project.org/vocab/ro#annotation-3 -->

    <owl:NamedIndividual rdf:about="&ro;annotation-3">
        <rdf:type rdf:resource="&ao;Annotation"/>
        <ao:body rdf:resource="&ro;annotationBody-3"/>
        <dcmi-terms:creator rdf:resource="&ro;user-18933"/>
        <ao:annotatesResource rdf:resource="&ro;workflow-run"/>
    </owl:NamedIndividual>
    


    <!-- http://www.wf4ever-project.org/vocab/ro#annotation-4 -->

    <owl:NamedIndividual rdf:about="&ro;annotation-4">
        <rdf:type rdf:resource="&ao;Annotation"/>
        <ao:body rdf:resource="&ro;annotationBody-4"/>
        <dcmi-terms:creator rdf:resource="&ro;user-18933"/>
        <ao:annotatesResource rdf:resource="&ro;workflow-run"/>
    </owl:NamedIndividual>
    


    <!-- http://www.wf4ever-project.org/vocab/ro#annotation-5 -->

    <owl:NamedIndividual rdf:about="&ro;annotation-5">
        <rdf:type rdf:resource="&ao;Annotation"/>
        <ao:body rdf:resource="&ro;annotationBody-5"/>
        <dcmi-terms:creator rdf:resource="&ro;user-18933"/>
        <ao:annotatesResource rdf:resource="&ro;workflow-run"/>
    </owl:NamedIndividual>
    


    <!-- http://www.wf4ever-project.org/vocab/ro#annotation-6 -->

    <owl:NamedIndividual rdf:about="&ro;annotation-6">
        <rdf:type rdf:resource="&ao;Annotation"/>
        <ao:body rdf:resource="&ro;annotationBody-6"/>
        <ao:annotatesResource rdf:resource="&ro;workflow-run"/>
    </owl:NamedIndividual>
    


    <!-- http://www.wf4ever-project.org/vocab/ro#annotationBody-1 -->

    <owl:Thing rdf:about="&ro;annotationBody-1">
        <rdf:type rdf:resource="&owl;NamedIndividual"/>
        <rdfs:comment rdf:datatype="&rdf;PlainLiteral">This is a named graph that asserts that 

workflow-run1 used external-1</rdfs:comment>
    </owl:Thing>
    


    <!-- http://www.wf4ever-project.org/vocab/ro#annotationBody-2 -->

    <owl:Thing rdf:about="&ro;annotationBody-2">
        <rdf:type rdf:resource="&owl;NamedIndividual"/>
        <dcmi-terms:creator rdf:datatype="&rdf;PlainLiteral">This is a named graph that asserts that 

workflow-run1 used external-2</dcmi-terms:creator>
    </owl:Thing>
    


    <!-- http://www.wf4ever-project.org/vocab/ro#annotationBody-3 -->

    <owl:Thing rdf:about="&ro;annotationBody-3">
        <rdf:type rdf:resource="&owl;NamedIndividual"/>
        <rdfs:comment rdf:datatype="&rdf;PlainLiteral">This is a named graph that asserts that 

workflow-run1 used external-3</rdfs:comment>
    </owl:Thing>
    


    <!-- http://www.wf4ever-project.org/vocab/ro#annotationBody-4 -->

    <owl:Thing rdf:about="&ro;annotationBody-4">
        <rdf:type rdf:resource="&owl;NamedIndividual"/>
        <rdfs:comment rdf:datatype="&rdf;PlainLiteral">This is a named graph that asserts that 

file-576 wasGeneratedBy workflow-run1</rdfs:comment>
    </owl:Thing>
    


    <!-- http://www.wf4ever-project.org/vocab/ro#annotationBody-5 -->

    <owl:Thing rdf:about="&ro;annotationBody-5">
        <rdf:type rdf:resource="&owl;NamedIndividual"/>
        <rdfs:comment rdf:datatype="&rdf;PlainLiteral">This is a named graph that asserts that 

file-577 wasGeneratedBy workflow-run1</rdfs:comment>
    </owl:Thing>
    


    <!-- http://www.wf4ever-project.org/vocab/ro#annotationBody-6 -->

    <owl:Thing rdf:about="&ro;annotationBody-6">
        <rdf:type rdf:resource="&owl;NamedIndividual"/>
        <rdfs:comment>This is a named graph that asserts that 

workflow-run hasWorkflowTemplate workflow-2464</rdfs:comment>
    </owl:Thing>
    


    <!-- http://www.wf4ever-project.org/vocab/ro#external-1 -->

    <owl:NamedIndividual rdf:about="&ro;external-1">
        <rdf:type rdf:resource="&ns;Artifact"/>
        <rdfs:label rdf:datatype="&rdf;PlainLiteral">TSDL Home Page</rdfs:label>
        <rdfs:seeAlso rdf:datatype="&xsd;anyURI">http://robjhyndman.com/TSDL/</rdfs:seeAlso>
    </owl:NamedIndividual>
    


    <!-- http://www.wf4ever-project.org/vocab/ro#external-2 -->

    <owl:NamedIndividual rdf:about="&ro;external-2">
        <rdf:type rdf:resource="&ns;Artifact"/>
        <rdfs:label rdf:datatype="&rdf;PlainLiteral">Annual Unit Price of Lynx Pelts</rdfs:label>
        <rdfs:seeAlso rdf:datatype="&xsd;anyURI">http://robjhyndman.com/tsdldata/data/andrews3.dat</rdfs:seeAlso>
    </owl:NamedIndividual>
    


    <!-- http://www.wf4ever-project.org/vocab/ro#external-3 -->

    <owl:NamedIndividual rdf:about="&ro;external-3">
        <rdf:type rdf:resource="&ns;Artifact"/>
        <rdfs:label rdf:datatype="&rdf;PlainLiteral">Annual Number of Lynx Pelts</rdfs:label>
        <rdfs:seeAlso rdf:datatype="&xsd;anyURI">http://robjhyndman.com/tsdldata/data/andrews2.dat</rdfs:seeAlso>
    </owl:NamedIndividual>
    


    <!-- http://www.wf4ever-project.org/vocab/ro#files-576 -->

    <File rdf:about="&ro;files-576">
        <rdf:type rdf:resource="&owl;NamedIndividual"/>
        <rdfs:label rdf:datatype="&rdf;PlainLiteral">Google charts line chart result</rdfs:label>
    </File>
    


    <!-- http://www.wf4ever-project.org/vocab/ro#files-577 -->

    <File rdf:about="&ro;files-577">
        <rdf:type rdf:resource="&owl;NamedIndividual"/>
        <rdfs:label rdf:datatype="&rdf;PlainLiteral">Time Series Data Library Citation Result</rdfs:label>
    </File>
    


    <!-- http://www.wf4ever-project.org/vocab/ro#ro-217 -->

    <ResearchObject rdf:about="&ro;ro-217">
        <rdf:type rdf:resource="&owl;NamedIndividual"/>
        <rdfs:label rdf:datatype="&rdf;PlainLiteral">ResearchObject 217</rdfs:label>
        <rdfs:seeAlso rdf:datatype="&xsd;anyURI">http://www.myexperiment.org/packs/217</rdfs:seeAlso>
        <terms:aggregates rdf:resource="&ro;annotation-1"/>
        <terms:aggregates rdf:resource="&ro;annotation-2"/>
        <terms:aggregates rdf:resource="&ro;annotation-3"/>
        <terms:aggregates rdf:resource="&ro;annotation-4"/>
        <terms:aggregates rdf:resource="&ro;annotation-5"/>
        <terms:aggregates rdf:resource="&ro;external-1"/>
        <terms:aggregates rdf:resource="&ro;external-2"/>
        <terms:aggregates rdf:resource="&ro;external-3"/>
        <terms:aggregates rdf:resource="&ro;files-576"/>
        <terms:aggregates rdf:resource="&ro;files-577"/>
        <terms:aggregates rdf:resource="&ro;workflow-2464"/>
        <terms:aggregates rdf:resource="&ro;workflow-run"/>
    </ResearchObject>
    


    <!-- http://www.wf4ever-project.org/vocab/ro#user-18933 -->

    <owl:NamedIndividual rdf:about="&ro;user-18933">
        <rdfs:label rdf:datatype="&rdf;PlainLiteral">Tadamus</rdfs:label>
    </owl:NamedIndividual>
    


    <!-- http://www.wf4ever-project.org/vocab/ro#workflow-2464 -->

    <WorkflowTemplate rdf:about="&ro;workflow-2464">
        <rdf:type rdf:resource="&owl;NamedIndividual"/>
        <rdfs:label rdf:datatype="&rdf;PlainLiteral">Time Series Data Graphed and Cited</rdfs:label>
    </WorkflowTemplate>
    


    <!-- http://www.wf4ever-project.org/vocab/ro#workflow-run -->

    <WorkflowRun rdf:about="&ro;workflow-run">
        <rdf:type rdf:resource="&owl;NamedIndividual"/>
        <hasWorkflowTemplate rdf:resource="&ro;workflow-2464"/>
    </WorkflowRun>
</rdf:RDF>



<!-- Generated by the OWL API (version 3.0.0.1451) http://owlapi.sourceforge.net -->

