@prefix xsd: <http://www.w3.org/2001/XMLSchema#> .
@prefix owl: <http://www.w3.org/2002/07/owl#> .
@prefix : <http://www.wf4ever-project.org/vocab/ro#> .
@prefix xml: <http://www.w3.org/XML/1998/namespace> .
@prefix rdf: <http://www.w3.org/1999/02/22-rdf-syntax-ns#> .
@prefix rdfs: <http://www.w3.org/2000/01/rdf-schema#> .
@prefix skos: <http://www.w3.org/2004/02/skos/core#> .
@base <http://www.wf4ever-project.org/vocab/ro> .

<http://www.wf4ever-project.org/vocab/ro> rdf:type owl:Ontology ;
                                          
                                          owl:imports <http://purl.org/ao/> ,
                                                      <http://www.openarchives.org/ore/terms/> .


#################################################################
#
#    Annotation properties
#
#################################################################


rdfs:seeAlso rdf:type owl:AnnotationProperty .
rdfs:label rdf:type owl:AnnotationProperty .
rdfs:comment rdf:type owl:AnnotationProperty .
<http://dublincore.org/documents/dcmi-terms/creator> rdf:type owl:AnnotationProperty .


#################################################################
#
#    Datatypes
#
#################################################################


###  http://www.w3.org/1999/02/22-rdf-syntax-ns#PlainLiteral

rdf:PlainLiteral rdf:type rdfs:Datatype .





#################################################################
#
#    Object Properties
#
#################################################################


###  http://purl.org/ao/annotatesResource

<http://purl.org/ao/annotatesResource> rdf:type owl:ObjectProperty .



###  http://purl.org/ao/body

<http://purl.org/ao/body> rdf:type owl:ObjectProperty .



###  http://purl.org/net/opmv/ns#used

<http://purl.org/net/opmv/ns#used> rdf:type owl:ObjectProperty ;
                                   
                                   rdfs:comment "used associates an artifact with a process, specifying that the former was consumed by the latter." ;
                                   
                                   rdfs:range <http://purl.org/net/opmv/ns#Artifact> ;
                                   
                                   rdfs:domain <http://purl.org/net/opmv/ns#Process> ;
                                   
                                   rdfs:subPropertyOf owl:topObjectProperty .



###  http://purl.org/net/opmv/ns#wasControlledBy

<http://purl.org/net/opmv/ns#wasControlledBy> rdf:type owl:ObjectProperty ;
                                              
                                              rdfs:comment "wasControlledBy associates a process with an agent, specifying the process  was controlled, e.g., launched, suspended, or terminated, by the agent." ;
                                              
                                              rdfs:range <http://purl.org/net/opmv/ns#Agent> ;
                                              
                                              rdfs:domain <http://purl.org/net/opmv/ns#Process> ;
                                              
                                              rdfs:subPropertyOf owl:topObjectProperty .



###  http://purl.org/net/opmv/ns#wasGeneratedBy

<http://purl.org/net/opmv/ns#wasGeneratedBy> rdf:type owl:ObjectProperty ;
                                             
                                             rdfs:comment "wasGeneratedBy associates an artifact with a process, specifying that the former was produced by the latter." ;
                                             
                                             rdfs:domain <http://purl.org/net/opmv/ns#Artifact> ;
                                             
                                             rdfs:range <http://purl.org/net/opmv/ns#Process> ;
                                             
                                             rdfs:subPropertyOf owl:topObjectProperty .



###  http://www.openarchives.org/ore/terms/aggregates

<http://www.openarchives.org/ore/terms/aggregates> rdf:type owl:ObjectProperty .



###  http://www.w3.org/2002/07/owl#topObjectProperty

owl:topObjectProperty rdf:type owl:ObjectProperty .



###  http://www.wf4ever-project.org/vocab/ro#contains

:contains rdf:type owl:ObjectProperty ;
          
          rdfs:comment "This property associates a workflow run with a process to specify that the latter is a constituent of the former." ;
          
          rdfs:range <http://purl.org/net/opmv/ns#Process> ;
          
          rdfs:subPropertyOf owl:topObjectProperty ;
          
          rdfs:domain :WorkflowRun .



###  http://www.wf4ever-project.org/vocab/ro#hasArtifactTemplate

:hasArtifactTemplate rdf:type owl:ObjectProperty ;
                     
                     rdfs:comment "This object property is used to associate an artifact to its correponding template." ;
                     
                     rdfs:domain <http://purl.org/net/opmv/ns#Artifact> ;
                     
                     rdfs:subPropertyOf owl:topObjectProperty ;
                     
                     rdfs:range :ArtifactTemplate .



###  http://www.wf4ever-project.org/vocab/ro#hasInput

:hasInput rdf:type owl:ObjectProperty ;
          
          rdfs:comment "This object property is used to specify the template of the artifacts used as input to a given process template." ;
          
          rdfs:range :ArtifactTemplate ;
          
          rdfs:domain :ProcessTemplate .



###  http://www.wf4ever-project.org/vocab/ro#hasOutput

:hasOutput rdf:type owl:ObjectProperty ;
           
           rdfs:comment "This object property is used to specify the template of the artifacts used as output to a given process template." ;
           
           rdfs:range :ArtifactTemplate ;
           
           rdfs:domain :ProcessTemplate .



###  http://www.wf4ever-project.org/vocab/ro#hasProcessTemplate

:hasProcessTemplate rdf:type owl:ObjectProperty ;
                    
                    rdfs:comment "This object property associate a process to its template." ;
                    
                    rdfs:domain <http://purl.org/net/opmv/ns#Process> ;
                    
                    rdfs:subPropertyOf owl:topObjectProperty ;
                    
                    rdfs:range :ProcessTemplate .



###  http://www.wf4ever-project.org/vocab/ro#hasWorkflowTemplate

:hasWorkflowTemplate rdf:type owl:ObjectProperty ;
                     
                     rdfs:comment "This property associates a workflow run to its corresponding workflow template." ;
                     
                     rdfs:domain :WorkflowRun ;
                     
                     rdfs:range :WorkflowTemplate ;
                     
                     rdfs:subPropertyOf :hasProcessTemplate .



###  http://www.wf4ever-project.org/vocab/ro#isPartOf

:isPartOf rdf:type owl:ObjectProperty ;
          
          rdfs:comment "This object property is used to specify that a given process template is part of a given workflow template."^^rdf:PlainLiteral ;
          
          rdfs:subPropertyOf owl:topObjectProperty ;
          
          rdfs:domain :ProcessTemplate ;
          
          rdfs:range :WorkflowTemplate .



###  http://www.wf4ever-project.org/vocab/ro#isSubWorkflowOf

:isSubWorkflowOf rdf:type owl:ObjectProperty ;
                 
                 rdfs:comment "This object property is used to associate a workflow template to another workflow template, specifying that the former is a sub-workflow of the latter." ;
                 
                 rdfs:range :WorkflowTemplate ;
                 
                 rdfs:domain :WorkflowTemplate ;
                 
                 rdfs:subPropertyOf :isPartOf .



###  http://www.wf4ever-project.org/vocab/ro#wasEnactedBy

:wasEnactedBy rdf:type owl:ObjectProperty ;
              
              rdfs:comment "wasEnactedBy associates a process with a workflow engine, specifying that the execution of the former was enacted by the latter." ;
              
              rdfs:subPropertyOf <http://purl.org/net/opmv/ns#wasControlledBy> ;
              
              rdfs:range [ rdf:type owl:Restriction ;
                           owl:onProperty :wasEnactedBy ;
                           owl:someValuesFrom :WorkflowEngine
                         ] ;
              
              rdfs:domain [ rdf:type owl:Restriction ;
                            owl:onProperty :wasEnactedBy ;
                            owl:someValuesFrom <http://purl.org/net/opmv/ns#Process>
                          ] .



###  http://www.wf4ever-project.org/vocab/ro#wasSpecifiedUsing

:wasSpecifiedUsing rdf:type owl:ObjectProperty ;
                   
                   rdfs:comment "This object property is used to specify the workflow workbench using which a given workflow template was specified." ;
                   
                   rdfs:subPropertyOf owl:topObjectProperty ;
                   
                   rdfs:domain :WorkflowTemplate ;
                   
                   rdfs:range :WorkflowWorkbench .





#################################################################
#
#    Classes
#
#################################################################


###  http://purl.org/ao/Annotation

<http://purl.org/ao/Annotation> rdf:type owl:Class .



###  http://purl.org/net/opmv/ns#Agent

<http://purl.org/net/opmv/ns#Agent> rdf:type owl:Class ;
                                    
                                    owl:equivalentClass <http://xmlns.com/foaf/0.1/Agent> ;
                                    
                                    rdfs:comment "An agent represents the entity that can be used to control the execution of a process, is used to specify a workflow template, or is responsible for enacting a workflow run. " .



###  http://purl.org/net/opmv/ns#Artifact

<http://purl.org/net/opmv/ns#Artifact> rdf:type owl:Class ;
                                       
                                       rdfs:comment "Artifact is a general concept that represents immutable piece of state, which may have a physical embodiment in a physical object, or a digital representation in a computer system. Note, however, that in the context of the Wf4ever project, the focus is on artifact that are digital representations in a computer system." .



###  http://purl.org/net/opmv/ns#Process

<http://purl.org/net/opmv/ns#Process> rdf:type owl:Class ;
                                      
                                      rdfs:comment "Process refers to an action that may consume some existing arifacts, and may produce some new artifacts." .



###  http://www.openarchives.org/ore/terms/Aggregation

<http://www.openarchives.org/ore/terms/Aggregation> rdf:type owl:Class .



###  http://www.openarchives.org/ore/terms/ResourceMap

<http://www.openarchives.org/ore/terms/ResourceMap> rdf:type owl:Class .



###  http://www.w3.org/2002/07/owl#Thing

owl:Thing rdf:type owl:Class .



###  http://www.wf4ever-project.org/vocab/ro#ArtifactTemplate

:ArtifactTemplate rdf:type owl:Class ;
                  
                  rdfs:comment "ArtifactTemplate is used to provide information about a class of artifacts. For example, it can be used to specify the datatype of a dataset or the structure of a document." .



###  http://www.wf4ever-project.org/vocab/ro#Dataset

:Dataset rdf:type owl:Class ;
         
         rdfs:subClassOf <http://purl.org/net/opmv/ns#Artifact> .



###  http://www.wf4ever-project.org/vocab/ro#Document

:Document rdf:type owl:Class ;
          
          rdfs:subClassOf <http://purl.org/net/opmv/ns#Artifact> .



###  http://www.wf4ever-project.org/vocab/ro#File

:File rdf:type owl:Class ;
      
      rdfs:subClassOf <http://purl.org/net/opmv/ns#Artifact> .



###  http://www.wf4ever-project.org/vocab/ro#Image

:Image rdf:type owl:Class ;
       
       rdfs:subClassOf <http://purl.org/net/opmv/ns#Artifact> .



###  http://www.wf4ever-project.org/vocab/ro#Manifest

:Manifest rdf:type owl:Class ;
          
          rdfs:subClassOf <http://www.openarchives.org/ore/terms/ResourceMap> ;
          
          rdfs:comment "Manifest is used to describe a research object." .



###  http://www.wf4ever-project.org/vocab/ro#ProcessTemplate

:ProcessTemplate rdf:type owl:Class ;
                 
                 rdfs:comment "A process template is used to describe a class of actions that when enacted give rise to processes. " .



###  http://www.wf4ever-project.org/vocab/ro#ResearchObject

:ResearchObject rdf:type owl:Class ;
                
                rdfs:subClassOf <http://www.openarchives.org/ore/terms/Aggregation> ;
                
                rdfs:comment "A research object aggregates a number of resources. A resource can be a workflow, web service, document, data item, data set, workflow run, software or a research object." .



###  http://www.wf4ever-project.org/vocab/ro#Tool

:Tool rdf:type owl:Class ;
      
      rdfs:subClassOf <http://purl.org/net/opmv/ns#Agent> ;
      
      rdfs:comment "represents a software program" .



###  http://www.wf4ever-project.org/vocab/ro#WebServiceProcess

:WebServiceProcess rdf:type owl:Class ;
                   
                   rdfs:subClassOf :ProcessTemplate ;
                   
                   rdfs:comment "WebServiceProcess is a Process template, the enactment of which gives rise to a web service call." .



###  http://www.wf4ever-project.org/vocab/ro#WorkflowEngine

:WorkflowEngine rdf:type owl:Class ;
                
                rdfs:subClassOf :Tool ;
                
                rdfs:comment "A workflow engine is an egent that is responsible for enacting a given workflow template. The result of workflow enactment gives rise to a workflow run." .



###  http://www.wf4ever-project.org/vocab/ro#WorkflowResearchObject

:WorkflowResearchObject rdf:type owl:Class ;
                        
                        owl:equivalentClass [ rdf:type owl:Class ;
                                              owl:intersectionOf ( :ResearchObject
                                                                   [ rdf:type owl:Restriction ;
                                                                     owl:onProperty <http://www.openarchives.org/ore/terms/aggregates> ;
                                                                     owl:someValuesFrom :WorkflowTemplate
                                                                   ]
                                                                 )
                                            ] ;
                        
                        rdfs:comment "A workflow research object is a research object that contains at least one workflow template." .



###  http://www.wf4ever-project.org/vocab/ro#WorkflowRun

:WorkflowRun rdf:type owl:Class ;
             
             rdfs:subClassOf <http://purl.org/net/opmv/ns#Process> ;
             
             rdfs:comment "A workflow run is a special kind of process that is composed of a series of actions." .



###  http://www.wf4ever-project.org/vocab/ro#WorkflowTemplate

:WorkflowTemplate rdf:type owl:Class ;
                  
                  rdfs:subClassOf :ProcessTemplate ;
                  
                  rdfs:comment "A workflow template is a directed graph in which the nodes are process templates and the edges represent data dependencies between the constituent process templates." .



###  http://www.wf4ever-project.org/vocab/ro#WorkflowWorkbench

:WorkflowWorkbench rdf:type owl:Class ;
                   
                   rdfs:subClassOf :Tool ;
                   
                   rdfs:comment "A workflow workbench is a software program that provides designers with a a means to design workflow templates." .



###  http://xmlns.com/foaf/0.1/Agent

<http://xmlns.com/foaf/0.1/Agent> rdf:type owl:Class .





#################################################################
#
#    Individuals
#
#################################################################


###  http://www.wf4ever-project.org/vocab/ro#annotation-1

:annotation-1 rdf:type <http://purl.org/ao/Annotation> ,
                       owl:NamedIndividual ;
              
              <http://purl.org/ao/body> :annotationBody-1 ;
              
              <http://dublincore.org/documents/dcmi-terms/creator> :user-18933 ;
              
              <http://purl.org/ao/annotatesResource> :workflow-run .



###  http://www.wf4ever-project.org/vocab/ro#annotation-2

:annotation-2 rdf:type <http://purl.org/ao/Annotation> ,
                       owl:NamedIndividual ;
              
              <http://purl.org/ao/body> :annotationBody-2 ;
              
              <http://dublincore.org/documents/dcmi-terms/creator> :user-18933 ;
              
              <http://purl.org/ao/annotatesResource> :workflow-run .



###  http://www.wf4ever-project.org/vocab/ro#annotation-3

:annotation-3 rdf:type <http://purl.org/ao/Annotation> ,
                       owl:NamedIndividual ;
              
              <http://purl.org/ao/body> :annotationBody-3 ;
              
              <http://dublincore.org/documents/dcmi-terms/creator> :user-18933 ;
              
              <http://purl.org/ao/annotatesResource> :workflow-run .



###  http://www.wf4ever-project.org/vocab/ro#annotation-4

:annotation-4 rdf:type <http://purl.org/ao/Annotation> ,
                       owl:NamedIndividual ;
              
              <http://purl.org/ao/body> :annotationBody-4 ;
              
              <http://dublincore.org/documents/dcmi-terms/creator> :user-18933 ;
              
              <http://purl.org/ao/annotatesResource> :workflow-run .



###  http://www.wf4ever-project.org/vocab/ro#annotation-5

:annotation-5 rdf:type <http://purl.org/ao/Annotation> ,
                       owl:NamedIndividual ;
              
              <http://purl.org/ao/body> :annotationBody-5 ;
              
              <http://dublincore.org/documents/dcmi-terms/creator> :user-18933 ;
              
              <http://purl.org/ao/annotatesResource> :workflow-run .



###  http://www.wf4ever-project.org/vocab/ro#annotation-6

:annotation-6 rdf:type <http://purl.org/ao/Annotation> ,
                       owl:NamedIndividual ;
              
              <http://purl.org/ao/body> :annotationBody-6 ;
              
              <http://purl.org/ao/annotatesResource> :workflow-run .



###  http://www.wf4ever-project.org/vocab/ro#annotationBody-1

:annotationBody-1 rdf:type owl:NamedIndividual ,
                           owl:Thing ;
                  
                  rdfs:comment """This is a named graph that asserts that 

workflow-run1 used external-1"""^^rdf:PlainLiteral .



###  http://www.wf4ever-project.org/vocab/ro#annotationBody-2

:annotationBody-2 rdf:type owl:NamedIndividual ,
                           owl:Thing ;
                  
                  <http://dublincore.org/documents/dcmi-terms/creator> """This is a named graph that asserts that 

workflow-run1 used external-2"""^^rdf:PlainLiteral .



###  http://www.wf4ever-project.org/vocab/ro#annotationBody-3

:annotationBody-3 rdf:type owl:NamedIndividual ,
                           owl:Thing ;
                  
                  rdfs:comment """This is a named graph that asserts that 

workflow-run1 used external-3"""^^rdf:PlainLiteral .



###  http://www.wf4ever-project.org/vocab/ro#annotationBody-4

:annotationBody-4 rdf:type owl:NamedIndividual ,
                           owl:Thing ;
                  
                  rdfs:comment """This is a named graph that asserts that 

file-576 wasGeneratedBy workflow-run1"""^^rdf:PlainLiteral .



###  http://www.wf4ever-project.org/vocab/ro#annotationBody-5

:annotationBody-5 rdf:type owl:NamedIndividual ,
                           owl:Thing ;
                  
                  rdfs:comment """This is a named graph that asserts that 

file-577 wasGeneratedBy workflow-run1"""^^rdf:PlainLiteral .



###  http://www.wf4ever-project.org/vocab/ro#annotationBody-6

:annotationBody-6 rdf:type owl:NamedIndividual ,
                           owl:Thing ;
                  
                  rdfs:comment """This is a named graph that asserts that 

workflow-run hasWorkflowTemplate workflow-2464""" .



###  http://www.wf4ever-project.org/vocab/ro#external-1

:external-1 rdf:type <http://purl.org/net/opmv/ns#Artifact> ,
                     owl:NamedIndividual ;
            
            rdfs:label "TSDL Home Page"^^rdf:PlainLiteral ;
            
            rdfs:seeAlso "http://robjhyndman.com/TSDL/"^^xsd:anyURI .



###  http://www.wf4ever-project.org/vocab/ro#external-2

:external-2 rdf:type <http://purl.org/net/opmv/ns#Artifact> ,
                     owl:NamedIndividual ;
            
            rdfs:label "Annual Unit Price of Lynx Pelts"^^rdf:PlainLiteral ;
            
            rdfs:seeAlso "http://robjhyndman.com/tsdldata/data/andrews3.dat"^^xsd:anyURI .



###  http://www.wf4ever-project.org/vocab/ro#external-3

:external-3 rdf:type <http://purl.org/net/opmv/ns#Artifact> ,
                     owl:NamedIndividual ;
            
            rdfs:label "Annual Number of Lynx Pelts"^^rdf:PlainLiteral ;
            
            rdfs:seeAlso "http://robjhyndman.com/tsdldata/data/andrews2.dat"^^xsd:anyURI .



###  http://www.wf4ever-project.org/vocab/ro#files-576

:files-576 rdf:type owl:NamedIndividual ,
                    :File ;
           
           rdfs:label "Google charts line chart result"^^rdf:PlainLiteral .



###  http://www.wf4ever-project.org/vocab/ro#files-577

:files-577 rdf:type owl:NamedIndividual ,
                    :File ;
           
           rdfs:label "Time Series Data Library Citation Result"^^rdf:PlainLiteral .



###  http://www.wf4ever-project.org/vocab/ro#ro-217

:ro-217 rdf:type owl:NamedIndividual ,
                 :ResearchObject ;
        
        rdfs:label "ResearchObject 217"^^rdf:PlainLiteral ;
        
        rdfs:seeAlso "http://www.myexperiment.org/packs/217"^^xsd:anyURI ;
        
        <http://www.openarchives.org/ore/terms/aggregates> :annotation-1 ,
                                                           :annotation-2 ,
                                                           :annotation-3 ,
                                                           :annotation-4 ,
                                                           :annotation-5 ,
                                                           :external-1 ,
                                                           :external-2 ,
                                                           :external-3 ,
                                                           :files-576 ,
                                                           :files-577 ,
                                                           :workflow-2464 ,
                                                           :workflow-run .



###  http://www.wf4ever-project.org/vocab/ro#user-18933

:user-18933 rdf:type owl:NamedIndividual ;
            
            rdfs:label "Tadamus"^^rdf:PlainLiteral .



###  http://www.wf4ever-project.org/vocab/ro#workflow-2464

:workflow-2464 rdf:type owl:NamedIndividual ,
                        :WorkflowTemplate ;
               
               rdfs:label "Time Series Data Graphed and Cited"^^rdf:PlainLiteral .



###  http://www.wf4ever-project.org/vocab/ro#workflow-run

:workflow-run rdf:type owl:NamedIndividual ,
                       :WorkflowRun ;
              
              :hasWorkflowTemplate :workflow-2464 .




###  Generated by the OWL API (version 3.0.0.1451) http://owlapi.sourceforge.net

